Man zeigt A durch $\neg A \Rightarrow \text{Falsch}$
## Beispiel
$$
\begin{gather}
\text{Z.z.:} \, x, y \in \mathbb{Q}, \, x \cdot y \notin \mathbb{Q}, \, \Rightarrow x \notin \mathbb{Q} \, \lor \, y \notin \mathbb{Q}. \\ \\
\text{Beweis durch Widerspruch:} \\ \\
\text{Es existieren } \, a, b, c, d \in \mathbb{Z}, \
\text{so dass} \ x = \frac{a}{b} \quad \text{und} \quad y = \frac{c}{d}. \\ \\
\Rightarrow x \cdot y = \frac{a}{b} \cdot \frac{c}{d} = \frac{a \cdot c}{b \cdot d}. \\
\Rightarrow \, \frac{a \cdot c}{b \cdot d} \in \mathbb{Q}. \\ \\
\text{Widerspruch zu Annahme } \, x \cdot y \notin \mathbb{Q}. \\
\Rightarrow \, x \notin \mathbb{Q} \, \text{ oder } \, y \notin \mathbb{Q}. \quad \text{q.e.d.}
\end{gather}
$$


